src/lowparse/LowParse.SLow.Array.fst
@@ -1,6 +1,6 @@
 module LowParse.SLow.Array
 include LowParse.SLow.FLData
-include LowParse.SLow.VLData
+include LowParse.SLow.VLGen
 include LowParse.SLow.List
 include LowParse.Spec.Array
 
@@ -83,8 +83,11 @@ inline_for_extraction
 let parse32_vlarray
   (array_byte_size_min: nat)
   (array_byte_size_min32: U32.t { U32.v array_byte_size_min32 == array_byte_size_min } )
-  (array_byte_size_max: nat)
+  (array_byte_size_max: nat { array_byte_size_min <= array_byte_size_max } )
   (array_byte_size_max32: U32.t { U32.v array_byte_size_max32 == array_byte_size_max } )
+  (#hk: parser_kind)
+  (#hp: parser hk (bounded_int32 array_byte_size_min array_byte_size_max))
+  (hp32: parser32 hp)
   (#k: parser_kind)
   (#t: Type0)
   (#p: parser k t)
@@ -95,7 +98,7 @@ let parse32_vlarray
   (u: unit {
     vldata_vlarray_precond array_byte_size_min array_byte_size_max p elem_count_min elem_count_max == true  
   })
-: Tot (parser32 (parse_vlarray array_byte_size_min array_byte_size_max s elem_count_min elem_count_max u))
+: Tot (parser32 (parse_vlarray array_byte_size_min array_byte_size_max hp s elem_count_min elem_count_max u))
 = [@inline_let]
   let _ =
     vldata_to_vlarray_inj array_byte_size_min array_byte_size_max s elem_count_min elem_count_max u
@@ -104,11 +107,12 @@ let parse32_vlarray
     _
     (vldata_to_vlarray array_byte_size_min array_byte_size_max s elem_count_min elem_count_max u)
     (fun x -> vldata_to_vlarray array_byte_size_min array_byte_size_max s elem_count_min elem_count_max u x)
-    (parse32_bounded_vldata_strong
+    (parse32_bounded_vlgen
       array_byte_size_min
       array_byte_size_min32
       array_byte_size_max
       array_byte_size_max32
+      hp32
       (serialize_list _ s)
       (parse32_list p32)
     )
@@ -117,7 +121,11 @@ let parse32_vlarray
 inline_for_extraction
 let serialize32_vlarray
   (array_byte_size_min: nat)
-  (array_byte_size_max: nat { array_byte_size_max < 4294967292 } ) // NOTE here: max must be less than 2^32 - 4 to account for the size of the length header
+  (array_byte_size_max: nat { array_byte_size_min <= array_byte_size_max })
+  (#hk: parser_kind)
+  (#hp: parser hk (bounded_int32 array_byte_size_min array_byte_size_max))
+  (#hs: serializer hp)
+  (hs32: serializer32 hs { hk.parser_kind_subkind == Some ParserStrong /\ Some? hk.parser_kind_high /\ Some?.v hk.parser_kind_high + array_byte_size_max < 4294967296 } ) // size bound necessary for FStar.Bytes.concat
   (#k: parser_kind)
   (#t: Type0)
   (#p: parser k t)
@@ -128,7 +136,7 @@ let serialize32_vlarray
   (u: unit {
     vldata_vlarray_precond array_byte_size_min array_byte_size_max p elem_count_min elem_count_max == true  
   })
-: Tot (serializer32 (serialize_vlarray array_byte_size_min array_byte_size_max s elem_count_min elem_count_max u))
+: Tot (serializer32 (serialize_vlarray array_byte_size_min array_byte_size_max hs s elem_count_min elem_count_max u))
 = [@inline_let]
   let _ =
     vldata_to_vlarray_inj array_byte_size_min array_byte_size_max s elem_count_min elem_count_max u
@@ -141,9 +149,10 @@ let serialize32_vlarray
     _
     (vldata_to_vlarray array_byte_size_min array_byte_size_max s elem_count_min elem_count_max u)
     _
-    (serialize32_bounded_vldata_strong
+    (serialize32_bounded_vlgen
       array_byte_size_min
       array_byte_size_max
+      hs32
       (partial_serialize32_list _ _ s32 ())
     )
     (vlarray_to_vldata array_byte_size_min array_byte_size_max s elem_count_min elem_count_max u)
@@ -153,7 +162,11 @@ let serialize32_vlarray
 inline_for_extraction
 let size32_vlarray
   (array_byte_size_min: nat)
-  (array_byte_size_max: nat { array_byte_size_max < 4294967292 } ) // NOTE here: max must be less than 2^32 - 4 to account for the size of the length header
+  (array_byte_size_max: nat { array_byte_size_min <= array_byte_size_max } )
+  (#hk: parser_kind)
+  (#hp: parser hk (bounded_int32 array_byte_size_min array_byte_size_max))
+  (#hs: serializer hp)
+  (hs32: size32 hs { hk.parser_kind_subkind == Some ParserStrong })
   (#k: parser_kind)
   (#t: Type0)
   (#p: parser k t)
@@ -163,9 +176,8 @@ let size32_vlarray
   (u: unit {
     vldata_vlarray_precond array_byte_size_min array_byte_size_max p elem_count_min elem_count_max == true  
   })
-  (size_header_byte_size32: U32.t { U32.v size_header_byte_size32 == log256' array_byte_size_max } )
   (elem_byte_size32: U32.t { U32.v elem_byte_size32 == k.parser_kind_low } )
-: Tot (size32 (serialize_vlarray array_byte_size_min array_byte_size_max s elem_count_min elem_count_max u))
+: Tot (size32 (serialize_vlarray array_byte_size_min array_byte_size_max hs s elem_count_min elem_count_max u))
 = [@inline_let]
   let _ =
     vldata_to_vlarray_inj array_byte_size_min array_byte_size_max s elem_count_min elem_count_max u
@@ -177,12 +189,17 @@ let size32_vlarray
   size32_synth
     _
     (vldata_to_vlarray array_byte_size_min array_byte_size_max s elem_count_min elem_count_max u)
-    _
-    (size32_bounded_vldata_strong
+    (serialize_bounded_vlgen
       array_byte_size_min
       array_byte_size_max
+      hs
+      (serialize_list _ s)
+    )
+    (size32_bounded_vlgen
+      array_byte_size_min
+      array_byte_size_max
+      hs32
       (size32_list #_ #_ #_ #s (size32_constant s elem_byte_size32 ()) ())
-      size_header_byte_size32
     )
     (vlarray_to_vldata array_byte_size_min array_byte_size_max s elem_count_min elem_count_max u)
     (fun x -> vlarray_to_vldata array_byte_size_min array_byte_size_max s elem_count_min elem_count_max u x)
